

EMS702P Statistical Thinking and Applied Machine Learning

Week 9 – PBL Solutions

Yunpeng Zhu

Solution 1:

(a):

According to the initial settings of $\bar{w}_1 = 0.3$ and $\bar{w}_2 = 0.1$, the initial outputs of the neural network is

$$\begin{cases} \bar{z}_1(1) = \bar{w}_1 x(1) = 0.3 \times 1 = 0.3 \\ \bar{z}_1(2) = \bar{w}_1 x(2) = 0.3 \times 1.5 = 0.45 \\ \bar{z}_1(3) = \bar{w}_1 x(3) = 0.3 \times 2 = 0.6 \end{cases} \quad (1)$$

$$\begin{cases} f[\bar{z}_1(1)] = \frac{1}{1 + \exp[-\bar{z}_1(1)]} = \frac{1}{1 + \exp(-0.3)} = 0.574 \\ f[\bar{z}_1(2)] = \frac{1}{1 + \exp[-\bar{z}_1(2)]} = \frac{1}{1 + \exp(-0.45)} = 0.611 \\ f[\bar{z}_1(3)] = \frac{1}{1 + \exp[-\bar{z}_1(3)]} = \frac{1}{1 + \exp(-0.6)} = 0.646 \end{cases} \quad (2)$$

$$\begin{cases} \bar{y}(1) = \bar{z}_2(1) = \bar{w}_2 f[\bar{z}_1(1)] = 0.1 \times 0.574 = 0.0574 \\ \bar{y}(2) = \bar{z}_2(2) = \bar{w}_2 f[\bar{z}_1(2)] = 0.1 \times 0.611 = 0.0611 \\ \bar{y}(3) = \bar{z}_2(3) = \bar{w}_2 f[\bar{z}_1(3)] = 0.1 \times 0.646 = 0.0646 \end{cases} \quad (3)$$

The cost function of the neural network is

$$\begin{aligned} J &= \frac{J_1 + J_2 + J_3}{3} \\ &= \frac{1}{3} \left\{ \frac{1}{2} [\bar{y}(1) - y(1)]^2 + \frac{1}{2} [\bar{y}(2) - y(2)]^2 + \frac{1}{2} [\bar{y}(3) - y(3)]^2 \right\} \end{aligned} \quad (4)$$

Now calculate the gradients separately:

(b):

The gradient of J with respect to the weight w_2 is obtained as

$$\frac{\partial J}{\partial w_2} = \frac{1}{3} \left[\frac{\partial J_1}{\partial w_2} + \frac{\partial J_2}{\partial w_2} + \frac{\partial J_3}{\partial w_2} \right] \quad (5)$$

in which the gradients of J_t , $t = 1, 2, 3$ with respect to w_2 are obtained as

$$\frac{\partial J_t}{\partial w_2} = [\bar{y}(t) - y(t)] \times \frac{\partial y}{\partial w_2} \Big|_{y=y(t)}, k = 1, 2, 3 \quad (6)$$

where

$$\frac{\partial y}{\partial w_2} = \frac{\partial [f(z_1)w_2]}{\partial w_2} = f(z_1) \quad (7)$$

Therefore,

$$\begin{cases} \frac{\partial J_1}{\partial w_2} = [\bar{y}(1) - y(1)] f[\bar{z}_1(1)] = (0.0574 - 0.3) \times 0.574 = -0.139 \\ \frac{\partial J_2}{\partial w_2} = [\bar{y}(2) - y(2)] f[\bar{z}_1(2)] = (0.0611 - 0.6) \times 0.611 = -0.329 \\ \frac{\partial J_3}{\partial w_2} = [\bar{y}(3) - y(3)] f[\bar{z}_1(3)] = (0.0646 - 0.8) \times 0.646 = -0.475 \end{cases} \quad (8)$$

Substituting (8) into gradient (5), yields

$$\frac{\partial J}{\partial w_2} = \frac{1}{3} \times (-0.139 - 0.329 - 0.475) = -0.314 \quad (9)$$

(c):

The gradient of J with respect to the weight w_1 is obtained as

$$\frac{\partial J}{\partial w_1} = \frac{1}{3} \left[\frac{\partial J_1}{\partial w_1} + \frac{\partial J_2}{\partial w_1} + \frac{\partial J_3}{\partial w_1} \right] \quad (10)$$

in which the gradients of $J_t, t = 1, 2, 3$ with respect to w_1 is obtained as

$$\frac{\partial J_t}{\partial w_1} = [\bar{y}(t) - y(t)] \times \frac{\partial y}{\partial w_1} \Big|_{y=y(t)}, t = 1, 2, 3 \quad (11)$$

where

$$\frac{\partial y}{\partial w_1} = \frac{\partial z_2}{\partial w_1} = \frac{\partial z_2}{\partial f(z_1)} \frac{\partial f(z_1)}{\partial z_1} \frac{\partial z_1}{\partial w_1} \quad (12)$$

with

$$\frac{\partial z_2}{\partial f(z_1)} = \frac{\partial [w_2 f(z_1)]}{\partial f(z_1)} = w_2 \quad (13)$$

$$\frac{\partial f(z_1)}{\partial z_1} = f(z_1)(1 - f(z_1)) \quad (14)$$

$$\frac{\partial z_1}{\partial w_1} = \frac{\partial(w_1 x)}{\partial w_1} = x \quad (15)$$

Therefore,

$$\left\{ \begin{aligned} \frac{\partial J_1}{\partial w_1} &= [\bar{y}(1) - y(1)] \bar{w}_2 f[\bar{z}_1(1)] [1 - f[\bar{z}_1(1)]] x(1) \\ &= (0.0574 - 0.3) \times 0.1 \times 0.574 \times (1 - 0.574) \times 1 = -0.00593 \\ \frac{\partial J_1}{\partial w_2} &= [\bar{y}(2) - y(2)] \bar{w}_2 f[\bar{z}_1(2)] [1 - f[\bar{z}_1(2)]] x(2) \\ &= (0.0611 - 0.6) \times 0.1 \times 0.611 \times (1 - 0.611) \times 1.5 = -0.0192 \\ \frac{\partial J_1}{\partial w_3} &= [\bar{y}(3) - y(3)] \bar{w}_2 f[\bar{z}_1(3)] [1 - f[\bar{z}_1(3)]] x(3) \\ &= (0.0646 - 0.8) \times 0.1 \times 0.646 \times (1 - 0.646) \times 2 = -0.034 \end{aligned} \right. \quad (16)$$

Substituting (16) into gradient (10), yields

$$\frac{\partial J}{\partial w_1} = \frac{1}{3} \times (-0.00593 - 0.0192 - 0.034) = -0.0197 \quad (17)$$

(d):

The weights w_2 and w_1 can be updated by using the gradient decent approach as

$$\begin{aligned} w_2 &= \bar{w}_2 - \lambda \frac{\partial J}{\partial w_2} = 0.1 + 0.5 \times 0.314 = 0.257 \\ w_1 &= \bar{w}_1 - \lambda \frac{\partial J}{\partial w_1} = 0.3 + 0.5 \times 0.0197 = 0.31 \end{aligned} \quad (18)$$

Solution 2:

Step 1: Determine the weight matrices

$$\mathbf{W}^{[2]} = \begin{bmatrix} w_{0,1}^{[2]} & w_{0,2}^{[2]} & w_{0,3}^{[2]} \\ \vdots & \vdots & \vdots \\ w_{4,1}^{[2]} & w_{4,2}^{[2]} & w_{4,3}^{[2]} \end{bmatrix}, \mathbf{W}^{[1]} = \begin{bmatrix} w_{0,1}^{[1]} & \cdots & w_{0,4}^{[1]} \\ \vdots & \ddots & \vdots \\ w_{8,1}^{[1]} & \cdots & w_{8,4}^{[1]} \end{bmatrix}$$

Step 2: Calculate the output layer gradient

$$\nabla \mathbf{J}_{\mathbf{w}^{[2]}} = \begin{bmatrix} \frac{\partial J_1}{\partial w_{0,1}^{[2]}} & \dots & \frac{\partial J_3}{\partial w_{0,4}^{[2]}} \\ \vdots & \ddots & \vdots \\ \frac{\partial J_1}{\partial w_{8,1}^{[2]}} & \dots & \frac{\partial J_3}{\partial w_{8,4}^{[2]}} \end{bmatrix} = [(\hat{\mathbf{Y}} - \mathbf{Y})\mathbf{H}^T]^T$$

where

$$\hat{\mathbf{Y}} - \mathbf{Y} = \begin{bmatrix} \frac{\partial J_1}{\partial \hat{y}_1} \\ \frac{\partial J_2}{\partial \hat{y}_2} \\ \frac{\partial J_3}{\partial \hat{y}_3} \end{bmatrix}, \quad \mathbf{H} = \begin{bmatrix} \frac{\partial \hat{y}_k}{\partial w_{0,k}^{[2]}} \\ \vdots \\ \frac{\partial \hat{y}_k}{\partial w_{4,k}^{[2]}} \end{bmatrix}$$

Step 3: Calculate the input layer gradient

$$\nabla \mathbf{J}_{\mathbf{w}^{[1]}} = \begin{bmatrix} \sum_{k=1}^3 \frac{\partial J_k}{\partial w_{0,1}^{[1]}} & \sum_{k=1}^3 \frac{\partial J_k}{\partial w_{0,2}^{[1]}} & \sum_{k=1}^3 \frac{\partial J_k}{\partial w_{0,3}^{[1]}} \\ \vdots & \vdots & \vdots \\ \sum_{k=1}^3 \frac{\partial J_k}{\partial w_{4,1}^{[1]}} & \sum_{k=1}^3 \frac{\partial J_k}{\partial w_{4,2}^{[1]}} & \sum_{k=1}^3 \frac{\partial J_k}{\partial w_{4,3}^{[1]}} \end{bmatrix}$$

$$= \left(\{[(\hat{\mathbf{Y}} - \mathbf{Y})^T (\bar{\mathbf{W}}^{[2]})^T]^T \odot \mathbf{H}_d\} \mathbf{X}^T \right)^T$$

where

$$\hat{\mathbf{Y}} - \mathbf{Y} = \begin{bmatrix} \frac{\partial J_1}{\partial \hat{y}_1} \\ \frac{\partial J_2}{\partial \hat{y}_2} \\ \frac{\partial J_3}{\partial \hat{y}_3} \end{bmatrix}, \quad \bar{\mathbf{W}}^{[2]} = \begin{bmatrix} \frac{\partial \hat{y}_1}{\partial h_1} & \frac{\partial \hat{y}_2}{\partial h_1} & \frac{\partial \hat{y}_3}{\partial h_1} \\ \vdots & \vdots & \vdots \\ \frac{\partial \hat{y}_1}{\partial h_4} & \frac{\partial \hat{y}_2}{\partial h_4} & \frac{\partial \hat{y}_3}{\partial h_4} \end{bmatrix} = \begin{bmatrix} w_{0,1}^{[2]} & w_{0,2}^{[2]} & w_{0,3}^{[2]} \\ \vdots & \vdots & \vdots \\ w_{4,1}^{[2]} & w_{4,2}^{[2]} & w_{4,3}^{[2]} \end{bmatrix},$$

$$\mathbf{H}_d = \begin{bmatrix} \frac{\partial h_1}{\partial z_1} \\ \vdots \\ \frac{\partial h_4}{\partial z_4} \end{bmatrix}, \quad \mathbf{X} = \begin{bmatrix} 1 \\ \vdots \\ x_8 \end{bmatrix}$$